src/tls/TLS.Handshake.Transcript.fst
@@ -401,7 +401,7 @@ let etx =
   else Ghost.erased transcript_t
 
 noeq
-type state (a:HashDef.hash_alg) = {
+type state (a:ha) = {
   region:Mem.rgn;
   loc: Ghost.erased B.loc;
   hash_state: CRF.state a;
@@ -413,7 +413,7 @@ let get_transcript #a (s:state a) (h:HS.mem) : GTot transcript_t =
   let etx = HS.sel h s.transcript in
   if transcript_idealization then etx else Ghost.reveal etx
 
-let invariant (#a:HashDef.hash_alg) (s:state a) (h:HS.mem) =
+let invariant (#a:ha) (s:state a) (h:HS.mem) =
   let tx = get_transcript s h in
   HS.contains h s.transcript /\
   CRF.hashed h s.hash_state `Seq.equal` transcript_bytes tx /\
@@ -425,7 +425,7 @@ let invariant (#a:HashDef.hash_alg) (s:state a) (h:HS.mem) =
   B.loc_disjoint (B.loc_region_only true Mem.tls_tables_region)
                  (B.loc_region_only true s.region)
 
-let footprint (#a:HashDef.hash_alg) (s:state a) = Ghost.reveal s.loc
+let footprint (#a:ha) (s:state a) = Ghost.reveal s.loc
 
 let transcript = get_transcript
 
@@ -433,7 +433,7 @@ let elim_invariant #a s h = ()
 
 let region_of #a s = s.region
 
-let frame_invariant (#a:_) (s:state a) (h0 h1:HS.mem) (l:B.loc) =
+let frame_invariant (#a:ha) (s:state a) (h0 h1:HS.mem) (l:B.loc) =
   CRF.frame_invariant l s.hash_state h0 h1
 
 let create r a =
@@ -827,13 +827,13 @@ let extend (#a:_) (s:state a) (l:label_repr) =
   | LR_HSM13 _ ->
     extend_hsm13 s l
 
-let transcript_hash (a:HashDef.hash_alg) (t:transcript_t)
+let transcript_hash (a:ha) (t:transcript_t)
   = Spec.Agile.Hash.hash a (transcript_bytes t)
 
-let hashed (a:HashDef.hash_alg) (t:transcript_t) =
+let hashed (a:ha) (t:transcript_t) =
   Model.CRF.hashed a (transcript_bytes t)
 
-let extract_hash (#a:_) (s:state a)
+let extract_hash (#a:ha) (s:state a)
   (tag:Hacl.Hash.Definitions.hash_t a)
   =
     let h0 = HyperStack.ST.get() in
